reflexivity for sim_ectx

theories/simplang/heapbij_refl.v
@@ -82,6 +82,9 @@ Section refl.
     iIntros "Hv Hs". destruct b; first done. by iApply (map_ForallI_insert_2 with "[Hv] Hs").
   Qed.
 
+  Lemma subst_map_rel_empty : ⊢ subst_map_rel ∅.
+  Proof. apply map_ForallI_empty. Qed.
+
   Definition sem_wf e_t e_s : iProp Σ :=
     ∀ (map : gmap string (val * val)),
       subst_map_rel map -∗ subst_map (fst <$> map) e_t ⪯ subst_map (snd <$> map) e_s {{ val_rel }}.
@@ -133,44 +136,44 @@ Section refl.
     source_stuck_prim.
   Qed.
 
-  Lemma sem_wf_let x e1 e2 :
-    sem_wf e1 e1 -∗ sem_wf e2 e2 -∗ sem_wf (Let x e1 e2) (Let x e1 e2).
+  Lemma sem_wf_let x e1_t e1_s e2_t e2_s :
+    sem_wf e1_t e1_s -∗ sem_wf e2_t e2_s -∗ sem_wf (Let x e1_t e2_t) (Let x e1_s e2_s).
   Proof.
     iIntros "IH1 IH2" (xs) "#Hs"; simpl.
-    smart_sim_bind (subst_map _ e1) (subst_map _ e1) "(IH1 Hs)".
+    smart_sim_bind (subst_map _ e1_t) (subst_map _ e1_s) "(IH1 Hs)".
     iIntros (v_t v_s) "#Hv". sim_pures. rewrite !subst'_subst_map.
     rewrite -(binder_insert_fmap fst (v_t, v_s)).
     rewrite -(binder_insert_fmap snd (v_t, v_s)).
     iApply "IH2". by iApply (subst_map_rel_insert with "Hv").
   Qed.
 
-  Lemma sem_wf_call e1 e2 :
-    sem_wf e1 e1 -∗ sem_wf e2 e2 -∗ sem_wf (Call e1 e2) (Call e1 e2).
+  Lemma sem_wf_call e1_t e1_s e2_t e2_s :
+    sem_wf e1_t e1_s -∗ sem_wf e2_t e2_s -∗ sem_wf (Call e1_t e2_t) (Call e1_s e2_s).
   Proof.
     iIntros "IH1 IH2" (xs) "#Hs"; simpl.
-    smart_sim_bind (subst_map _ e2) (subst_map _ e2) "(IH2 Hs)".
+    smart_sim_bind (subst_map _ e2_t) (subst_map _ e2_s) "(IH2 Hs)".
     iIntros (v_t1 v_s1) "#Hv1".
-    smart_sim_bind (subst_map _ e1) (subst_map _ e1) "(IH1 Hs)".
+    smart_sim_bind (subst_map _ e1_t) (subst_map _ e1_s) "(IH1 Hs)".
     iIntros (v_t2 v_s2) "#Hv2".
     discr_source; first by apply call_not_val. val_discr_source "Hv2".
     iApply sim_call; done.
   Qed.
 
-  Lemma sem_wf_unop e o :
-    sem_wf e e -∗ sem_wf (UnOp o e) (UnOp o e).
+  Lemma sem_wf_unop e_t e_s o :
+    sem_wf e_t e_s -∗ sem_wf (UnOp o e_t) (UnOp o e_s).
   Proof.
     iIntros "IH" (xs) "#Hs"; simpl.
-    smart_sim_bind (subst_map _ e) (subst_map _ e) "(IH Hs)".
+    smart_sim_bind (subst_map _ e_t) (subst_map _ e_s) "(IH Hs)".
     iIntros (v_t v_s) "#Hv". destruct o; sim_pures; discr_source; val_discr_source "Hv"; by sim_pures; sim_val.
   Qed.
 
-  Lemma sem_wf_binop e1 e2 o :
-    sem_wf e1 e1 -∗ sem_wf e2 e2 -∗ sem_wf (BinOp o e1 e2) (BinOp o e1 e2).
+  Lemma sem_wf_binop e1_t e1_s e2_t e2_s o :
+    sem_wf e1_t e1_s -∗ sem_wf e2_t e2_s -∗ sem_wf (BinOp o e1_t e2_t) (BinOp o e1_s e2_s).
   Proof.
     iIntros "IH1 IH2" (xs) "#Hs"; simpl.
-    smart_sim_bind (subst_map _ e2) (subst_map _ e2) "(IH2 Hs)".
+    smart_sim_bind (subst_map _ e2_t) (subst_map _ e2_s) "(IH2 Hs)".
     iIntros (v_t2 v_s2) "Hv2".
-    smart_sim_bind (subst_map _ e1) (subst_map _ e1) "(IH1 Hs)".
+    smart_sim_bind (subst_map _ e1_t) (subst_map _ e1_s) "(IH1 Hs)".
     iIntros (v_t1 v_s1) "Hv1".
     destruct o; sim_pures; discr_source; val_discr_source "Hv1"; val_discr_source "Hv2"; sim_pures; [sim_val; done .. | | ].
     - iAssert (⌜vals_compare_safe v_t1 v_t2⌝)%I as "%".
@@ -188,79 +191,79 @@ Section refl.
       by iApply heap_bij_loc_shift.
   Qed.
 
-  Lemma sem_wf_if e1 e2 e3 :
-    sem_wf e1 e1 -∗ sem_wf e2 e2 -∗ sem_wf e3 e3 -∗ sem_wf (If e1 e2 e3) (If e1 e2 e3).
+  Lemma sem_wf_if e1_t e1_s e2_t e2_s e3_t e3_s :
+    sem_wf e1_t e1_s -∗ sem_wf e2_t e2_s -∗ sem_wf e3_t e3_s -∗ sem_wf (If e1_t e2_t e3_t) (If e1_s e2_s e3_s).
   Proof.
     iIntros "IH1 IH2 IH3" (xs) "#Hs"; simpl.
-    smart_sim_bind (subst_map _ e1) (subst_map _ e1) "(IH1 Hs)".
+    smart_sim_bind (subst_map _ e1_t) (subst_map _ e1_s) "(IH1 Hs)".
     iIntros (v_t v_s) "Hv".
     discr_source. val_discr_source "Hv". destruct x; sim_pures.
     + iApply ("IH2" with "Hs").
     + iApply ("IH3" with "Hs").
   Qed.
 
-  Lemma sem_wf_while e1 e2 :
-    (□ sem_wf e1 e1) -∗ (□ sem_wf e2 e2) -∗ sem_wf (While e1 e2) (While e1 e2).
+  Lemma sem_wf_while e1_t e1_s e2_t e2_s :
+    (□ sem_wf e1_t e1_s) -∗ (□ sem_wf e2_t e2_s) -∗ sem_wf (While e1_t e2_t) (While e1_s e2_s).
   Proof.
     iIntros "#IH1 #IH2" (xs) "#Hs"; simpl.
     iApply (sim_while_while _ _ _ _ _ (True)%I with "[//]").
     iModIntro; iIntros "_".
-    smart_sim_bind (subst_map _ e1) (subst_map _ e1) "(IH1 Hs)".
+    smart_sim_bind (subst_map _ e1_t) (subst_map _ e1_s) "(IH1 Hs)".
     iIntros (v_t v_s) "Hv".
     discr_source. val_discr_source "Hv". destruct x; sim_pures.
-    + smart_sim_bind (subst_map _ e2) (subst_map _ e2) "(IH2 Hs)".
+    + smart_sim_bind (subst_map _ e2_t) (subst_map _ e2_s) "(IH2 Hs)".
       iIntros (? ?) "_"; sim_pures. iApply sim_expr_base. iRight. by eauto.
     + iApply sim_expr_base. iLeft. iExists #(), #(); eauto.
   Qed.
 
-  Lemma sem_wf_pair e1 e2 :
-    sem_wf e1 e1 -∗ sem_wf e2 e2 -∗ sem_wf (Pair e1 e2) (Pair e1 e2).
+  Lemma sem_wf_pair e1_t e1_s e2_t e2_s :
+    sem_wf e1_t e1_s -∗ sem_wf e2_t e2_s -∗ sem_wf (Pair e1_t e2_t) (Pair e1_s e2_s).
   Proof.
     iIntros "IH1 IH2" (xs) "#Hs"; simpl.
-    smart_sim_bind (subst_map _ e2) (subst_map _ e2) "(IH2 Hs)".
+    smart_sim_bind (subst_map _ e2_t) (subst_map _ e2_s) "(IH2 Hs)".
     iIntros (v_t2 v_s2) "Hv2".
-    smart_sim_bind (subst_map _ e1) (subst_map _ e1) "(IH1 Hs)".
+    smart_sim_bind (subst_map _ e1_t) (subst_map _ e1_s) "(IH1 Hs)".
     iIntros (v_t1 v_s1) "Hv1".
     sim_pures; sim_val. iModIntro; iSplit; eauto.
   Qed.
 
-  Lemma sem_wf_fst e :
-    sem_wf e e -∗ sem_wf (Fst e) (Fst e).
+  Lemma sem_wf_fst e_t e_s :
+    sem_wf e_t e_s -∗ sem_wf (Fst e_t) (Fst e_s).
   Proof.
     iIntros "IH" (xs) "#Hs"; simpl.
-    smart_sim_bind (subst_map _ e) (subst_map _ e) "(IH Hs)".
+    smart_sim_bind (subst_map _ e_t) (subst_map _ e_s) "(IH Hs)".
     iIntros (v_t v_s) "Hv".
     discr_source. iPoseProof (val_rel_pair_source with "Hv") as (??) "(-> & ? & ?)"; by sim_pures; sim_val.
   Qed.
-  Lemma sem_wf_snd e :
-    sem_wf e e -∗ sem_wf (Snd e) (Snd e).
+  Lemma sem_wf_snd e_t e_s :
+    sem_wf e_t e_s -∗ sem_wf (Snd e_t) (Snd e_s).
   Proof.
     iIntros "IH" (xs) "#Hs"; simpl.
-    smart_sim_bind (subst_map _ e) (subst_map _ e) "(IH Hs)".
+    smart_sim_bind (subst_map _ e_t) (subst_map _ e_s) "(IH Hs)".
     iIntros (v_t v_s) "Hv".
     discr_source. iPoseProof (val_rel_pair_source with "Hv") as (??) "(-> & ? & ?)"; by sim_pures; sim_val.
   Qed.
 
-  Lemma sem_wf_injl e :
-    sem_wf e e -∗ sem_wf (InjL e) (InjL e).
+  Lemma sem_wf_injl e_t e_s :
+    sem_wf e_t e_s -∗ sem_wf (InjL e_t) (InjL e_s).
   Proof.
     iIntros "IH" (xs) "#Hs"; simpl.
-    smart_sim_bind (subst_map _ e) (subst_map _ e) "(IH Hs)".
+    smart_sim_bind (subst_map _ e_t) (subst_map _ e_s) "(IH Hs)".
     iIntros (v_t v_s) "Hv"; by sim_pures; sim_val.
   Qed.
-  Lemma sem_wf_injr e :
-    sem_wf e e -∗ sem_wf (InjR e) (InjR e).
+  Lemma sem_wf_injr e_t e_s :
+    sem_wf e_t e_s -∗ sem_wf (InjR e_t) (InjR e_s).
   Proof.
     iIntros "IH" (xs) "#Hs"; simpl.
-    smart_sim_bind (subst_map _ e) (subst_map _ e) "(IH Hs)".
+    smart_sim_bind (subst_map _ e_t) (subst_map _ e_s) "(IH Hs)".
     iIntros (v_t v_s) "Hv"; by sim_pures; sim_val.
   Qed.
 
-  Lemma sem_wf_match e e1 e2 x1 x2 :
-    sem_wf e e -∗ sem_wf e1 e1 -∗ sem_wf e2 e2 -∗ sem_wf (Match e x1 e1 x2 e2) (Match e x1 e1 x2 e2).
+  Lemma sem_wf_match e_t e_s e1_t e1_s e2_t e2_s x1 x2 :
+    sem_wf e_t e_s -∗ sem_wf e1_t e1_s -∗ sem_wf e2_t e2_s -∗ sem_wf (Match e_t x1 e1_t x2 e2_t) (Match e_s x1 e1_s x2 e2_s).
   Proof.
     iIntros "IH IH1 IH2" (xs) "#Hs"; simpl.
-    smart_sim_bind (subst_map _ e) (subst_map _ e)  "(IH Hs)".
+    smart_sim_bind (subst_map _ e_t) (subst_map _ e_s)  "(IH Hs)".
     iIntros (v_t v_s) "#Hv".
     discr_source.
     + iPoseProof (val_rel_injl_source with "Hv") as (v_t') "(-> & ?)". sim_pures.
@@ -275,20 +278,20 @@ Section refl.
       iApply "IH2". by iApply subst_map_rel_insert.
   Qed.
 
-  Lemma sem_wf_fork e :
-    sem_wf e e -∗ sem_wf (Fork e) (Fork e).
+  Lemma sem_wf_fork e_t e_s :
+    sem_wf e_t e_s -∗ sem_wf (Fork e_t) (Fork e_s).
   Proof.
     iIntros "IH" (xs) "#Hs"; simpl.
     iApply sim_fork; first by sim_pures; sim_val. sim_pures.
     iApply (sim_wand with "(IH Hs)"). eauto.
   Qed.
 
-  Lemma sem_wf_allocN e1 e2 :
-    sem_wf e1 e1 -∗ sem_wf e2 e2 -∗ sem_wf (AllocN e1 e2) (AllocN e1 e2).
+  Lemma sem_wf_allocN e1_t e1_s e2_t e2_s :
+    sem_wf e1_t e1_s -∗ sem_wf e2_t e2_s -∗ sem_wf (AllocN e1_t e2_t) (AllocN e1_s e2_s).
   Proof.
     iIntros "IH1 IH2" (xs) "#Hs"; simpl.
-    smart_sim_bind (subst_map _ e2) (subst_map _ e2) "(IH2 Hs)". iIntros (v_t v_s) "Hv".
-    smart_sim_bind (subst_map _ e1) (subst_map _ e1) "(IH1 Hs)". iIntros (v_t' v_s') "Hv'".
+    smart_sim_bind (subst_map _ e2_t) (subst_map _ e2_s) "(IH2 Hs)". iIntros (v_t v_s) "Hv".
+    smart_sim_bind (subst_map _ e1_t) (subst_map _ e1_s) "(IH1 Hs)". iIntros (v_t' v_s') "Hv'".
     discr_source. val_discr_source "Hv'".
     target_alloc l_t as "Hl_t" "Ha_t"; first done.
     source_alloc l_s as "Hl_s" "Ha_s"; first done.
@@ -301,42 +304,52 @@ Section refl.
     iIntros "Hv". sim_pures. sim_val. done.
   Qed.
 
-  Lemma sem_wf_freeN e1 e2 :
-    sem_wf e1 e1 -∗ sem_wf e2 e2 -∗ sem_wf (FreeN e1 e2) (FreeN e1 e2).
+  Lemma sem_wf_freeN e1_t e1_s e2_t e2_s :
+    sem_wf e1_t e1_s -∗ sem_wf e2_t e2_s -∗ sem_wf (FreeN e1_t e2_t) (FreeN e1_s e2_s).
   Proof.
     iIntros "IH1 IH2" (xs) "#Hs"; simpl.
-    smart_sim_bind (subst_map _ e2) (subst_map _ e2) "(IH2 Hs)". iIntros (v_t v_s) "Hv".
-    smart_sim_bind (subst_map _ e1) (subst_map _ e1) "(IH1 Hs)". iIntros (v_t' v_s') "Hv'".
+    smart_sim_bind (subst_map _ _) (subst_map _ _) "(IH2 Hs)". iIntros (v_t v_s) "Hv".
+    smart_sim_bind (subst_map _ _) (subst_map _ _) "(IH1 Hs)". iIntros (v_t' v_s') "Hv'".
     discr_source. iPoseProof (val_rel_loc_source with "Hv") as (l_t) "(-> & Hrel)".
     iPoseProof (val_rel_litint_source with "Hv'") as "->".
     by sim_free; sim_val.
   Qed.
 
-  Lemma sem_wf_load o e :
-    sem_wf e e -∗ sem_wf (Load o e) (Load o e).
+  Lemma sem_wf_load o e_t e_s :
+    sem_wf e_t e_s -∗ sem_wf (Load o e_t) (Load o e_s).
   Proof.
     iIntros "IH" (xs) "#Hs"; simpl.
-    smart_sim_bind (subst_map _ e) (subst_map _ e) "(IH Hs)".
+    smart_sim_bind (subst_map _ _) (subst_map _ _) "(IH Hs)".
     iIntros (v_t v_s) "Hv". discr_source. iPoseProof (val_rel_loc_source with "Hv") as (l_t) "(-> & Hrel)".
     by sim_load v_t v_s as "Hv"; sim_val.
   Qed.
 
-  Lemma sem_wf_store o e1 e2 :
-    sem_wf e1 e1 -∗ sem_wf e2 e2 -∗ sem_wf (Store o e1 e2) (Store o e1 e2).
+  Lemma sem_wf_store o e1_t e1_s e2_t e2_s :
+    sem_wf e1_t e1_s -∗ sem_wf e2_t e2_s -∗ sem_wf (Store o e1_t e2_t) (Store o e1_s e2_s).
   Proof.
     iIntros "IH1 IH2" (xs) "#Hs"; simpl.
-    smart_sim_bind (subst_map _ e2) (subst_map _ e2) "(IH2 Hs)".
+    smart_sim_bind (subst_map _ _) (subst_map _ _) "(IH2 Hs)".
     iIntros (v_t v_s) "Hv". (* FIXME: fix printing *)
-    smart_sim_bind (subst_map _ e1) (subst_map _ e1) "(IH1 Hs)".
+    smart_sim_bind (subst_map _ _) (subst_map _ _) "(IH1 Hs)".
     iIntros (v_t' v_s') "Hv'".
     discr_source. iPoseProof (val_rel_loc_source with "Hv'") as (l_t) "(-> & Hrel)".
     by sim_store; [done | sim_val].
   Qed.
 
+  Lemma sem_wf_val v_t v_s :
+    val_rel v_t v_s -∗ sem_wf (Val v_t) (Val v_s).
+  Proof. iIntros "Hv" (xs) "#Hs"; simpl. by sim_val. Qed.
+
+  Lemma sem_wf_empty e_t e_s : sem_wf e_t e_s -∗ e_t ⪯ e_s {{ val_rel }}.
+  Proof.
+    iIntros "Hwf". iSpecialize ("Hwf" $! ∅ subst_map_rel_empty).
+    by rewrite !fmap_empty !subst_map_empty.
+  Qed.
+
   Lemma expr_wf_sound e : expr_wf e → ⊢ sem_wf e e.
   Proof.
     intros Hwf. iInduction e as [ ] "IH" forall (Hwf); iIntros (xs) "#Hs"; simpl.
-    - (* Val *) sim_pures; sim_val. iModIntro; by iApply val_wf_sound.
+    - (* Val *) iApply sem_wf_val; [by iApply val_wf_sound | done].
     - (* Var *) by iApply sem_wf_var.
     - (* Let *) destruct Hwf as [Hwf1 Hwf2]. by iApply (sem_wf_let with "(IH [//]) (IH1 [//])").
     - (* Call *) destruct Hwf as [Hwf1 Hwf2]. by iApply (sem_wf_call with "(IH [//]) (IH1 [//])").
@@ -367,4 +380,75 @@ Section refl.
     rewrite !subst_map_empty. iApply "Hwf". rewrite /subst_map_rel.
     by rewrite -map_ForallI_empty.
   Qed.
+
+  Definition ectxi_wf (Ki : ectx_item) : Prop :=
+    match Ki with
+    | LetCtx _ e => expr_wf e
+    | UnOpCtx _ => True
+    | BinOpLCtx _ v => val_wf v
+    | BinOpRCtx _ e => expr_wf e
+    | IfCtx e1 e2 => expr_wf e1 ∧ expr_wf e2
+    | PairLCtx v => val_wf v
+    | PairRCtx e => expr_wf e
+    | FstCtx | SndCtx | InjLCtx | InjRCtx | LoadCtx _ => True
+    | MatchCtx _ e1 _ e2 => expr_wf e1 ∧ expr_wf e2
+    | AllocNLCtx v => val_wf v
+    | AllocNRCtx e => expr_wf e
+    | FreeNLCtx v => val_wf v
+    | FreeNRCtx e => expr_wf e
+    | StoreLCtx _ v => val_wf v
+    | StoreRCtx _ e => expr_wf e
+    | CmpXchgLCtx _ _ => False  (* unsupported *)
+    | CmpXchgMCtx _ _ => False  (* unsupported *)
+    | CmpXchgRCtx _ _ => False  (* unsupported *)
+    | FaaLCtx _ => False  (* unsupported *)
+    | FaaRCtx _ => False (* unsupported *)
+    | CallLCtx v => val_wf v
+    | CallRCtx e => expr_wf e
+    end.
+  (* we do not use [Forall] since that does not compute,
+    making applications of [heap_bij_ectx_refl] hard. *)
+  Fixpoint ectx_wf (K : ectx) : Prop :=
+    match K with
+    | [] => True
+    | Ki :: K => ectxi_wf Ki ∧ ectx_wf K
+    end.
+
+  Theorem heap_bij_ectx_refl K :
+    ectx_wf K → ⊢ sim_ectx val_rel K K val_rel.
+  Proof.
+    intros Hwf. iInduction (K) as [ | Ki K] "IH".
+    { iIntros (v_t v_s) "Hv". sim_pures. by sim_val. }
+    destruct Hwf as [Hiwf Kwf].
+    iSpecialize ("IH" with "[//]").
+    iIntros (v_t v_s) "#Hv". destruct Ki; sim_pures; iApply sim_bind; (iApply sim_wand; [ iApply sem_wf_empty | iApply "IH"]).
+    - iApply sem_wf_let; [by iApply sem_wf_val | by iApply expr_wf_sound].
+    - iApply sem_wf_unop. by iApply sem_wf_val.
+    - iApply sem_wf_binop; [by iApply sem_wf_val | by iApply expr_wf_sound].
+    - iApply sem_wf_binop; [ by iApply expr_wf_sound | by iApply sem_wf_val].
+    - iApply sem_wf_if; [by iApply sem_wf_val | iApply expr_wf_sound; apply Hiwf..].
+    - iApply sem_wf_pair; iApply sem_wf_val; [done | by iApply val_wf_sound].
+    - iApply sem_wf_pair; [by iApply expr_wf_sound | by iApply sem_wf_val].
+    - iApply sem_wf_fst; by iApply sem_wf_val.
+    - iApply sem_wf_snd; by iApply sem_wf_val.
+    - iApply sem_wf_injl; by iApply sem_wf_val.
+    - iApply sem_wf_injr; by iApply sem_wf_val.
+    - iApply sem_wf_match; [by iApply sem_wf_val | iApply expr_wf_sound; apply Hiwf..].
+    - iApply sem_wf_allocN; [by iApply sem_wf_val | iApply sem_wf_val; by iApply val_wf_sound].
+    - iApply sem_wf_allocN; [iApply expr_wf_sound; apply Hiwf | by iApply sem_wf_val ].
+    - iApply sem_wf_freeN; [by iApply sem_wf_val | iApply expr_wf_sound; apply Hiwf].
+    - iApply sem_wf_freeN; [iApply expr_wf_sound; apply Hiwf | by iApply sem_wf_val ].
+    - iApply sem_wf_load; by iApply sem_wf_val.
+    - iApply sem_wf_store; [by iApply sem_wf_val | iApply expr_wf_sound; apply Hiwf].
+    - iApply sem_wf_store; [iApply expr_wf_sound; apply Hiwf | by iApply sem_wf_val ].
+    - by destruct Hiwf.
+    - by destruct Hiwf.
+    - by destruct Hiwf.
+    - by destruct Hiwf.
+    - by destruct Hiwf.
+    - iApply sem_wf_call; [by iApply sem_wf_val | iApply expr_wf_sound; apply Hiwf].
+    - iApply sem_wf_call; [iApply expr_wf_sound; apply Hiwf | by iApply sem_wf_val ].
+  Qed.
+
+  (* TODO: do the same thing for a general notion of contexts *)
 End refl.
